glue/rsa/bv256_ntt_lemmas.i.dfy
@@ -1,11 +1,11 @@
 include "../arch/otbn/machine.s.dfy"
 include "../arch/otbn/vale.i.dfy"
 
-include "bv256_ops.dfy"
+include "bv256_op_s.dfy"
 include "generic_ntt_lemmas.dfy"
 
 module bv256_ntt_lemmas refines generic_ntt_lemmas {
-    import opened GBV = bv256_ops
+    import opened GBV = bv256_op_s
     
     import opened ot_vale
     import opened ot_machine
