glue/rsa/bv32_falcon_lemmas.i.dfy
@@ -1,7 +1,7 @@
 include "../../arch/riscv/machine.s.dfy"
 include "../../arch/riscv/vale.i.dfy"
 include "ct_std2rev_model.dfy"
-include "../bv32_ops.dfy"
+include "../bv32_op_s.dfy"
 
 include "mq_arith_lemmas.dfy"
 include "../DivModNeg.dfy"
@@ -14,7 +14,7 @@ module bv32_falcon_lemmas {
     import opened Mul
     import opened DivModNeg
     import opened integers
-    import opened bv32_ops
+    import opened bv32_op_s
     import opened rv_machine
     import opened rv_vale
     import opened mem
