glue/rsa/bv32_ntt_lemmas.i.dfy
@@ -1,13 +1,13 @@
 include "../arch/riscv/machine.s.dfy"
 include "../arch/riscv/vale.i.dfy"
 
-include "bv32_ops.dfy"
+include "bv32_op_s.dfy"
 
 include "generic_ntt_lemmas.dfy"
 include "DivModNeg.dfy"
 
 module bv32_ntt_lemmas refines generic_ntt_lemmas {
-    import opened GBV = bv32_ops
+    import opened GBV = bv32_op_s
 
     import opened rv_machine
     import opened rv_vale
